SELFOUR-276: Add MCP to specs and invariants
A thread's maximum controlled priority (MCP) determines the maximum
thread priority or MCP it can assign to another thread (or itself).

spec/haskell/src/SEL4/API/Invocation.lhs
@@ -60,6 +60,7 @@ The following data type defines the set of possible TCB invocation operations. T
 >             tcThread :: PPtr TCB,
 >             tcThreadCapSlot :: PPtr CTE,
 >             tcNewFaultEP :: Maybe CPtr,
+>             tcNewMCPriority :: Maybe Priority,
 >             tcNewPriority :: Maybe Priority,
 >             tcNewCRoot, tcNewVRoot :: Maybe (Capability, PPtr CTE),
 >             tcNewIPCBuffer :: Maybe (VPtr, Maybe (Capability, PPtr CTE)) }
