spec/abstract/Decode_A.thy
@@ -212,19 +212,45 @@ where
 | _ \<Rightarrow> throwError TruncatedMessage"
 
 
+definition check_prio
+  :: "priority \<Rightarrow> obj_ref \<Rightarrow> (unit,'z::state_ext) se_monad" where
+  "check_prio new_prio cur \<equiv>
+    do
+      mcp \<leftarrow> thread_get tcb_mcpriority cur;
+      whenE (new_prio > mcp) $ throwError (RangeError 0 (ucast mcp))      
+    od"
+definition check_mcp
+  :: "priority \<Rightarrow> obj_ref \<Rightarrow> (unit,'z::state_ext) se_monad" where
+  "check_mcp new_mcp cur \<equiv>
+    do
+      mcp \<leftarrow> thread_get tcb_mcpriority cur;
+      check_prio mcp cur;
+      whenE (new_mcp > maxPrio) $ throwError (RangeError 0 (ucast maxPrio))
+    od"    
+
+
 definition
   decode_set_priority :: "data list \<Rightarrow> cap \<Rightarrow> cslot_ptr \<Rightarrow> (tcb_invocation,'z::state_ext) se_monad"
 where
   "decode_set_priority args cap slot \<equiv> 
      if length args = 0 then throwError TruncatedMessage
-     else doE
+     else let prio = (ucast $ args ! 0) in doE
        cur \<leftarrow> liftE $ gets cur_thread;
-       OR_choice (decode_set_priority_error_choice (ucast $ args ! 0) cur)
-           (throwError IllegalOperation)
-           (returnOk (ThreadControl (obj_ref_of cap) slot None
-             (Some (ucast $ args ! 0)) None None None))
+       check_prio prio cur;
+       returnOk (ThreadControl (obj_ref_of cap) slot None
+             (Some prio) None None None None)
+    odE"
+definition
+  decode_set_mcpriority :: "data list \<Rightarrow> cap \<Rightarrow> cslot_ptr \<Rightarrow> (tcb_invocation,'z::state_ext) se_monad"
+where
+  "decode_set_mcpriority args cap slot \<equiv> 
+     if length args = 0 then throwError TruncatedMessage
+     else let new_mcp = ucast $ args ! 0 in doE
+       cur \<leftarrow> liftE $ gets cur_thread;
+       check_mcp new_mcp cur;
+       returnOk (ThreadControl (obj_ref_of cap) slot None
+             None (Some new_mcp)None None None)
      odE"
-
 
 definition
   decode_set_ipc_buffer :: 
@@ -242,7 +268,7 @@ where
       returnOk $ Some (buffer_cap, bslot)
     odE;
   returnOk $ 
-    ThreadControl (obj_ref_of cap) slot None None None None (Some (buffer, newbuf))
+    ThreadControl (obj_ref_of cap) slot None None None None None (Some (buffer, newbuf))
 odE"
 
 
@@ -279,9 +305,15 @@ where
    unlessE (is_valid_vtable_root vroot_cap') $ throwError IllegalOperation;
    vroot \<leftarrow> returnOk (vroot_cap', vroot_slot);       
    
-   returnOk $ ThreadControl (obj_ref_of cap) slot (Some (to_bl fault_ep)) None 
+   returnOk $ ThreadControl (obj_ref_of cap) slot (Some (to_bl fault_ep)) None None
                             (Some croot) (Some vroot) None
  odE"
+
+definition prio_from_word :: "data \<Rightarrow> data" where
+"prio_from_word w \<equiv> ucast w"
+
+definition mcp_from_word :: "data \<Rightarrow> data" where
+"mcp_from_word w \<equiv> ucast (shiftr w 8)"
 
 
 definition
@@ -292,17 +324,18 @@ where
      whenE (length args < 5) $ throwError TruncatedMessage;
      whenE (length extra_caps < 3) $ throwError TruncatedMessage;
      fault_ep \<leftarrow> returnOk $ args ! 0;
-     prio     \<leftarrow> returnOk $ args ! 1;
+     prioProps  \<leftarrow> returnOk $ args ! 1;
      croot_data \<leftarrow> returnOk $ args ! 2;
      vroot_data \<leftarrow> returnOk $ args ! 3;
      crootvroot \<leftarrow> returnOk $ take 2 extra_caps;
      buffer_cap \<leftarrow> returnOk $ extra_caps ! 2;
      buffer \<leftarrow> returnOk $ args ! 4;
-     set_prio \<leftarrow> decode_set_priority [prio] cap slot;
+     set_prio \<leftarrow> decode_set_priority [prio_from_word prioProps] cap slot;
+     set_mcp \<leftarrow> decode_set_mcpriority [mcp_from_word prioProps] cap slot;
      set_params \<leftarrow> decode_set_ipc_buffer [buffer] cap slot [buffer_cap];
      set_space \<leftarrow> decode_set_space [fault_ep, croot_data, vroot_data] cap slot crootvroot;
      returnOk $ ThreadControl (obj_ref_of cap) slot (tc_new_fault_ep set_space)
-                              (tc_new_priority set_prio)
+                              (tc_new_priority set_prio) (tc_new_mcpriority set_mcp)
                               (tc_new_croot set_space) (tc_new_vroot set_space) 
                               (tc_new_buffer set_params)
    odE" 
@@ -359,6 +392,7 @@ where
     | TCBResume \<Rightarrow> returnOk $ Resume $ obj_ref_of cap
     | TCBConfigure \<Rightarrow> decode_tcb_configure args cap slot excs
     | TCBSetPriority \<Rightarrow> decode_set_priority args cap slot 
+    | TCBSetMCPriority \<Rightarrow> decode_set_mcpriority args cap slot
     | TCBSetIPCBuffer \<Rightarrow> decode_set_ipc_buffer args cap slot excs
     | TCBSetSpace \<Rightarrow> decode_set_space args cap slot excs
     | TCBBindNotification \<Rightarrow> decode_bind_notification cap excs
