proof/invariant-abstract/Include_AI.thy
@@ -44,6 +44,6 @@ crunch_ignore (add:
 crunch_ignore (add:
   cap_swap_ext cap_move_ext cap_insert_ext empty_slot_ext create_cap_ext tcb_sched_action
   reschedule_required set_thread_state_ext switch_if_required_to
-  attempt_switch_to timer_tick set_priority retype_region_ext)
+  attempt_switch_to timer_tick set_priority set_mcpriority retype_region_ext)
 
 end
