spec/abstract/ARM/Init_A.thy
@@ -80,7 +80,8 @@ definition
     tcb_ipc_buffer = 0,
     tcb_context = empty_context,
     tcb_fault = None,
-    tcb_bound_notification = None
+    tcb_bound_notification = None,
+    tcb_mcpriority = minBound
   \<rparr>, 
   init_globals_frame \<mapsto> ArchObj (DataPage False ARMSmallPage),
   init_global_pd \<mapsto> ArchObj (PageDirectory global_pd)
